NeverStarvation proof complete.

LeanLTL/Examples/TrafficLights.lean
@@ -11,9 +11,7 @@ open scoped LeanLTL.Notation
 
 -- Traffic Light Example
 structure ExState where
-  TL1Red: Prop
   TL1Green: Prop
-  TL2Red: Prop
   TL2Green: Prop
 
   TL1Arrives : ℕ
@@ -24,9 +22,7 @@ structure ExState where
   TL2Queue : ℕ
 
 abbrev TL1Green := LeanLTL.TraceSet.of ExState.TL1Green
-abbrev TL1Red := LeanLTL.TraceSet.of ExState.TL1Red
 abbrev TL2Green := LeanLTL.TraceSet.of ExState.TL2Green
-abbrev TL2Red := LeanLTL.TraceSet.of ExState.TL2Red
 abbrev TL1Arrives := LeanLTL.TraceFun.of ExState.TL1Arrives
 abbrev TL1Departs := LeanLTL.TraceFun.of ExState.TL1Departs
 abbrev TL2Arrives := LeanLTL.TraceFun.of ExState.TL2Arrives
@@ -38,19 +34,19 @@ abbrev max_arrives : ℕ := 2
 abbrev max_departs : ℕ := 2
 
 -- Base Properties
+-- TODO: Get rid of red prop
 abbrev TL1StartGreen    := LLTL[TL1Green]
-abbrev TL2StartRed      := LLTL[TL2Red]
+abbrev TL2StartRed      := LLTL[¬TL2Green]
 
-abbrev TL1GreenRedIff   := LLTL[G (TL1Green ↔ (¬TL1Red))]
-abbrev TL2GreenRedIff   := LLTL[G (TL2Green ↔ (¬TL2Red))]
-
-abbrev TL1ToTL2Green    := LLTL[G ((TL1Green ∧ ((← TL1Queue) == 0)) ↔ ((TL2Red ∧ TL1Green) ∧ (Xˢ (TL1Red ∧ TL2Green))))]
-abbrev TL2ToTL1Green    := LLTL[G ((TL2Green ∧ ((← TL2Queue) == 0)) ↔ ((TL1Red ∧ TL2Green) ∧ (Xˢ (TL2Red ∧ TL1Green))))]
+abbrev TL1ToTL2Green    := LLTL[G ((TL1Green ∧ ((← TL1Queue) == 0)) → (Xˢ (¬TL1Green ∧ TL2Green)))]
+abbrev TL2ToTL1Green    := LLTL[G ((TL2Green ∧ ((← TL2Queue) == 0)) → (Xˢ (TL1Green ∧ ¬ TL2Green)))]
+abbrev TL1StayGreen     := LLTL[G ((TL1Green ∧ ((← TL1Queue) != 0)) → (Xˢ (TL1Green ∧ ¬ TL2Green)))]
+abbrev TL2StayGreen     := LLTL[G ((TL2Green ∧ ((← TL2Queue) != 0)) → (Xˢ (¬ TL1Green ∧ TL2Green)))]
 
 abbrev TL1GreenDeparts  := LLTL[G (TL1Green → ((← TL1Departs) == max_departs))]
-abbrev TL1RedDeparts    := LLTL[G (TL1Red → ((← TL1Departs) == 0))]
+abbrev TL1RedDeparts    := LLTL[G (¬TL1Green → ((← TL1Departs) == 0))]
 abbrev TL2GreenDeparts  := LLTL[G (TL2Green → ((← TL2Departs) == max_departs))]
-abbrev TL2RedDeparts    := LLTL[G (TL2Red → ((← TL2Departs) == 0))]
+abbrev TL2RedDeparts    := LLTL[G (¬TL2Green → ((← TL2Departs) == 0))]
 
 abbrev TL1ArrivesBounds := LLTL[G (0 ≤ (← TL1Arrives) ∧ (← TL1Arrives) ≤ max_arrives)]
 abbrev TL2ArrivesBounds := LLTL[G (0 ≤ (← TL2Arrives) ∧ (← TL2Arrives) ≤ max_arrives)]
@@ -58,8 +54,8 @@ abbrev TL2ArrivesBounds := LLTL[G (0 ≤ (← TL2Arrives) ∧ (← TL2Arrives) �
 abbrev TL1QueueNext     := LLTL[G ((X (← TL1Queue)) == (← TL1Queue) + (← TL1Arrives) - (← TL1Departs))]
 abbrev TL2QueueNext     := LLTL[G ((X (← TL2Queue)) == (← TL2Queue) + (← TL2Arrives) - (← TL2Departs))]
 
-abbrev TLBaseProperties := LLTL[TL1StartGreen ∧ TL2StartRed ∧ TL1GreenRedIff ∧ TL2GreenRedIff
-                            ∧ TL1ToTL2Green ∧ TL2ToTL1Green ∧ TL1GreenDeparts ∧ TL1RedDeparts
+abbrev TLBaseProperties := LLTL[TL1StartGreen ∧ TL2StartRed ∧ TL1ToTL2Green ∧ TL2ToTL1Green
+                            ∧ TL1StayGreen ∧ TL2StayGreen ∧ TL1GreenDeparts ∧ TL1RedDeparts
                             ∧ TL2GreenDeparts ∧ TL2RedDeparts ∧ TL1ArrivesBounds ∧ TL2ArrivesBounds
                             ∧ TL1QueueNext ∧ TL2QueueNext]
 
@@ -67,7 +63,7 @@ abbrev TLBaseProperties := LLTL[TL1StartGreen ∧ TL2StartRed ∧ TL1GreenRedIff
 abbrev TrafficLulls       := LLTL[(G (F ((← TL1Arrives) == 0))) ∧ (G (F ((← TL2Arrives) == 0)))]
 
 -- Goal Properties
-abbrev LightSafety        := LLTL[G (TL1Green ↔ ¬TL2Green)]
+abbrev LightSafety        := LLTL[G (¬(TL1Green ∧ TL2Green))]
 abbrev NeverStarvation    := LLTL[(G (F ((← TL1Queue) == 0))) ∧ (G (F ((← TL2Queue) == 0)))]
 
 -- Example Proofs
@@ -76,42 +72,25 @@ theorem SatisfiesLightSafety : TLBaseProperties ⇒ⁱ LightSafety := by
   intro t h_t_inf h
   simp [LeanLTL.TraceSet.sat_and_iff] at h
   rcases h with ⟨h1, h2, h3, h4, h5, h6, h7, h8, h9, h10, h11, h12, h13, h14⟩
-  simp [LightSafety]
-
-  apply LeanLTL.TraceSet.globally_induction
-  . simp_all [push_fltl]
-    by_contra; rename_i contra
-    specialize h4 0 (by simp)
-    simp_all
-  . simp [push_fltl]
-    intro n h_n h15 h_n_1
-    simp [push_fltl] at *
-
-    by_cases h_ls_change : (t.shift n h_n) ⊨ LLTL[TL1Green == (Xˢ TL1Green)]
-    . simp [push_fltl] at h_ls_change
-      have : 1+n = n+1 := by omega
-      simp [this]
-      sorry
-
-    by_cases h_last_state: t.shift n h_n ⊨ TL1Green
-    . have h_last_state' := h15.mp h_last_state
-      simp [*] at h_last_state'
+  have h_ind : t ⊨ LLTL[G ((¬(TL1Green ∧ TL2Green)) ∧ (TL1Green ∨ TL2Green))] := by
+    apply LeanLTL.TraceSet.globally_induction
+    . simp [push_fltl] at h1 h2 ⊢
+      tauto
+    . simp [push_fltl] at h3 h4 h5 h6 ⊢
+      intro n h_n ih h_1_n h15
+      specialize h3 n h_n
+      specialize h4 n h_n
       specialize h5 n h_n
-      by_cases h_switch: (t.shift n h_n)⊨LLTL[TL1Queue == 0]
-      . have := h5.mp
-        specialize this (by simp_all)
-        rcases this with ⟨h17, h18⟩
-        specialize h18 h_n_1
-        simp_all
-      . have : ¬(((t.shift n h_n ⊨ TL1Green) ∧ t.shift n h_n ⊨ TL1Queue.eq (LeanLTL.TraceFun.const 0))) := by simp_all
-        simp [this, h15, h_last_state, h_switch] at h5
-        simp_all
-        specialize h3 (1+n) sorry
-        specialize h4 (1+n) sorry
+      specialize h6 n h_n
+      simp [*] at h3 h4 h5 h6
+      by_cases t.shift n h_n ⊨ TL1Green <;> by_cases t.shift n h_n ⊨ LLTL[((← TL1Queue) != 0)] <;> (simp_all; try tauto)
+  simp [push_fltl] at h_ind ⊢
+  simp_all
 
-        sorry
+theorem TrafficLullsImpliesNeverStarvation : LLTL[TrafficLulls ∧ TLBaseProperties] ⇒ⁱ NeverStarvation := by
+  simp [TLBaseProperties, LeanLTL.TraceSet.sem_imp_inf_iff, LeanLTL.TraceSet.sat_imp_iff]
+  intro t h_t_inf h
+  simp [LeanLTL.TraceSet.sat_and_iff] at h
+  rcases h with ⟨h1, h2, h3, h4, h5, h6, h7, h8, h9, h10, h11, h12, h13, h14, h15⟩
 
-      sorry
-    . sorry
-
-theorem TrafficLullsImpliesNeverStarvation : LLTL[TrafficLulls ∧ TLBaseProperties] ⇒ NeverStarvation := sorry
+  sorry
